code/k256/Hacl.Impl.K256.GLV.fst
@@ -13,10 +13,12 @@ module LSeq = Lib.Sequence
 module BE = Hacl.Impl.Exponentiation
 module ME = Hacl.Impl.MultiExponentiation
 module PM = Hacl.Impl.K256.PointMul
+module PT = Hacl.Impl.PrecompTable
 
 module S = Spec.K256
 module SG = Hacl.Spec.K256.GLV
 module SGL = Hacl.Spec.K256.GLV.Lemmas
+module SE = Spec.Exponentiation
 
 open Hacl.K256.Field
 open Hacl.K256.Scalar
@@ -25,7 +27,6 @@ open Hacl.Impl.K256.Point
 open Hacl.Impl.K256.GLV.Constants
 
 #set-options "--z3rlimit 50 --fuel 0 --ifuel 0"
-
 
 inline_for_extraction noextract
 val scalar_split_lambda_g1g2 (tmp1 tmp2 k1 k2 k: qelem) : Stack unit
@@ -108,6 +109,23 @@ let point_mul_lambda res p =
   copy_felem rz pz;
   pop_frame ()
 
+// [lambda]P = (beta * px, py, pz)
+inline_for_extraction noextract
+val point_mul_lambda_inplace: res:point -> Stack unit
+  (requires fun h ->
+    live h res /\ point_inv h res)
+  (ensures  fun h0 _ h1 -> modifies (loc res) h0 h1 /\
+    point_inv h1 res /\
+    point_eval h1 res == SG.point_mul_lambda (point_eval h0 res))
+
+let point_mul_lambda_inplace res =
+  push_frame ();
+  let rx, ry, rz = getx res, gety res, getz res in
+  let beta = create_felem () in
+  make_beta beta;
+  fmul rx beta rx;
+  pop_frame ()
+
 
 // // TODO: set it to a constant?
 // // [lambda]G
@@ -125,6 +143,83 @@ let point_mul_lambda res p =
 //   point_mul_lambda res g;
 //   pop_frame ()
 
+inline_for_extraction noextract
+let table1_inv_precomp (q:LSeq.lseq uint64 15) : BE.table_inv_t U64 15ul 16ul =
+  fun a table ->
+    point_eval_lseq a = SG.point_mul_lambda (point_eval_lseq q) /\
+    (forall (j:nat{j < 16}).
+      PT.precomp_table_inv 15ul 0ul PM.mk_k256_concrete_ops q 16ul table j)
+
+// This function returns [r_small]([lambda]Q)
+// using a precomputed table [0; Q; 2Q; ...; 15Q]
+inline_for_extraction noextract
+val lprecomp_get_consttime_lambda:
+  q:Ghost.erased (LSeq.lseq uint64 15){point_inv_lseq q} ->
+  BE.pow_a_to_small_b_st U64 15ul 0ul PM.mk_k256_concrete_ops 4ul 16ul (table1_inv_precomp q)
+
+let lprecomp_get_consttime_lambda q ctx lambda_q table1 r_small res =
+  let h0 = ST.get () in
+  assert (table1_inv_precomp q lambda_q (as_seq h0 table1));
+  // table1.[r_small] = [r_small]Q
+  BE.lprecomp_get_consttime 15ul 0ul PM.mk_k256_concrete_ops 4ul 16ul ctx q table1 r_small res;
+  let h1 = ST.get () in
+  assert (point_eval h1 res == SE.pow S.mk_k256_concrete_ops (point_eval_lseq q) (v r_small));
+  point_mul_lambda_inplace res;
+  let h2 = ST.get () in
+  assert (point_eval h2 res == SG.point_mul_lambda (point_eval h1 res));
+  // GLV lemma
+  assume (point_eval h2 res ==
+    SE.pow S.mk_k256_concrete_ops (point_eval_lseq lambda_q) (v r_small))
+
+
+inline_for_extraction noextract
+val point_mul_split_lambda_table: out:point -> r1:qelem -> r2:qelem -> q:point -> Stack unit
+  (requires fun h ->
+    live h out /\ live h r1 /\ live h r2 /\ live h q /\
+    disjoint out q /\ disjoint out r1 /\ disjoint out r2 /\
+    disjoint q r1 /\ disjoint q r2 /\
+    point_inv h q /\
+    qas_nat h r1 < S.q /\ qas_nat h r1 < pow2 129 /\
+    qas_nat h r2 < S.q /\ qas_nat h r2 < pow2 129)
+  (ensures  fun h0 _ h1 -> modifies (loc out) h0 h1 /\
+    point_inv h1 out /\
+    point_eval h1 out ==
+      SE.exp_double_fw S.mk_k256_concrete_ops (point_eval h0 q) 129
+        (qas_nat h0 r1) (SG.point_mul_lambda (point_eval h0 q)) (qas_nat h0 r2) 4)
+
+let point_mul_split_lambda_table out r1 r2 q =
+  let h0 = ST.get () in
+  push_frame ();
+  let q2 = create_point () in
+  point_mul_lambda q2 q; // q2 = [lambda]Q
+
+  [@inline_let] let len = 15ul in
+  [@inline_let] let ctx_len = 0ul in
+  [@inline_let] let k = PM.mk_k256_concrete_ops in
+  [@inline_let] let l = 4ul in
+  [@inline_let] let table_len = 16ul in
+  [@inline_let] let bLen = 4ul in
+  [@inline_let] let bBits = 129ul in
+
+  let table1 = create (table_len *! len) (u64 0) in
+  PT.lprecomp_table len ctx_len k (null uint64) q table_len table1;
+
+  ME.mk_lexp_double_fw_tables len ctx_len k l table_len
+    (BE.table_inv_precomp len ctx_len k l table_len)
+    (table1_inv_precomp (as_seq h0 q))
+    (BE.lprecomp_get_consttime len ctx_len k l table_len)
+    (lprecomp_get_consttime_lambda (as_seq h0 q))
+    (null uint64) q bLen bBits r1 q2 r2 table1 table1 out;
+
+  //ME.lexp_double_fw_vartime 15ul 0ul PM.mk_k256_concrete_ops 4ul (null uint64)
+    //q 4ul 129ul r1 q2 r2 out;
+  let h1 = ST.get () in
+  assert (point_eval h1 out ==
+      SE.exp_double_fw S.mk_k256_concrete_ops (point_eval h0 q) 129
+        (qas_nat h0 r1) (SG.point_mul_lambda (point_eval h0 q)) (qas_nat h0 r2) 4);
+  pop_frame ()
+
+
 // TODO: share a table [0; P; 2P; ..; 15P] between P and ([lambda]P)
 // [scalar]Q = [(r1 + r2 * lambda) % S.q]Q = [r1]Q + [r2]([lambda]Q)
 val point_mul_split_lambda: out:point -> scalar:qelem -> q:point -> Stack unit
@@ -140,15 +235,10 @@ val point_mul_split_lambda: out:point -> scalar:qelem -> q:point -> Stack unit
 let point_mul_split_lambda out scalar q =
   let h0 = ST.get () in
   push_frame ();
-  let q2 = create_point () in
-  point_mul_lambda q2 q;
-
   let r1 = create_qelem () in
   let r2 = create_qelem () in
-  scalar_split_lambda r1 r2 scalar;
-
-  ME.lexp_double_fw_vartime 15ul 0ul PM.mk_k256_concrete_ops 4ul (null uint64)
-    q 4ul 129ul r1 q2 r2 out;
+  scalar_split_lambda r1 r2 scalar; // (r1 + r2 * lambda) % S.q = scalar
+  point_mul_split_lambda_table out r1 r2 q;
 
   assume (
     SGL.point_mul_split_lambda (qas_nat h0 scalar) (point_eval h0 q) ==
