code/bignum/Hacl.Impl.PrecompTable.fsti
@@ -82,21 +82,20 @@ let lprecomp_get_st
   (len:size_t{v len > 0})
   (ctx_len:size_t)
   (k:concrete_ops a_t len ctx_len) =
-    a:lbuffer (uint_t a_t SEC) len
+    a:Ghost.erased (LSeq.lseq (uint_t a_t SEC) (v len))
   -> table_len:size_t{1 < v table_len /\ v table_len * v len <= max_size_t}
   -> table:lbuffer (uint_t a_t SEC) (table_len *! len)
   -> bits_l:uint_t a_t SEC{v bits_l < v table_len}
   -> tmp:lbuffer (uint_t a_t SEC) len ->
   Stack unit
   (requires fun h ->
-    live h a /\ live h table /\ live h tmp /\
-    disjoint a table /\ disjoint a tmp /\ disjoint table tmp /\
-    k.to.linv (as_seq h a) /\
+    live h table /\ live h tmp /\ disjoint table tmp /\
+    k.to.linv a /\
     (forall (j:nat{j < v table_len}).
-      precomp_table_inv len ctx_len k (as_seq h a) table_len (as_seq h table) j))
+      precomp_table_inv len ctx_len k a table_len (as_seq h table) j))
   (ensures  fun h0 _ h1 -> modifies (loc tmp) h0 h1 /\
     k.to.linv (as_seq h1 tmp) /\
-    k.to.refl (as_seq h1 tmp) == SE.pow k.to.concr_ops (k.to.refl (as_seq h0 a)) (v bits_l))
+    k.to.refl (as_seq h1 tmp) == SE.pow k.to.concr_ops (k.to.refl a) (v bits_l))
 
 
 // This function returns table.[bits_l] = a^bits_l
